nola/examples/logic/verify/na_ilist.v
@@ -5,40 +5,40 @@ From nola.iris Require Export wp.
 From nola.examples.heap_lang Require Export proofmode notation.
 
 (** Infinite list whose elements satisfy the condition [Φ] *)
-Definition na_ilist {κ Γᵘ Γᵍ} (p : na_inv_pool_name) (N N' : namespace)
+Definition na_ilist {κ Γᵘ Γᵍ} (p : na_inv_pool_name) (N : namespace)
   (Φ : loc → nPropL (;ᵞ Γᵘ ++ Γᵍ)) : loc → nProp κ (Γᵘ;ᵞ Γᵍ) :=
   (rec:ˢ l, n_na_inv' (_::_) p N (¢ᵍ Φ l) ∗
-    n_na_inv' (_::_) p N' (∃ l' : loc, (l +ₗ 1) ↦ # l' ∗ %ᵍˢ 0@ l'))%n.
+    n_na_inv' (_::_) p N (∃ l' : loc, (l +ₗ 1) ↦ # l' ∗ %ᵍˢ 0@ l'))%n.
 
 (** Substitution over [na_ilist] *)
-Fact na_ilist_nsubst {κ p N N' V Φ Ψ l} :
-  na_ilist (κ:=κ) (Γᵘ:=[V]) p N N' Φ l /: Ψ =
-    na_ilist (Γᵘ:=[]) p N N' (λ l, Φ l /:ᵍ Ψ) l.
+Fact na_ilist_nsubst {κ p N V Φ Ψ l} :
+  na_ilist (κ:=κ) (Γᵘ:=[V]) p N Φ l /: Ψ =
+    na_ilist (Γᵘ:=[]) p N (λ l, Φ l /:ᵍ Ψ) l.
 Proof. done. Qed.
 
 (** Interpreted [ilist] *)
-Definition na_ilisttl {κ} p N N' (Φ : _ → _ (;ᵞ)) l : nProp κ (;ᵞ) :=
-  ∃ l' : loc, (l +ₗ 1) ↦ # l' ∗ na_ilist (Γᵘ:=[]) p N N' Φ l'.
-Definition na_ilisti `{!nintpGS Σ} d p N N' Φ l : iProp Σ :=
-  na_nninv d p N (Φ l) ∗ na_nninv d p N' (na_ilisttl p N N' Φ l).
+Definition na_ilisttl {κ} p N (Φ : _ → _ (;ᵞ)) l : nProp κ (;ᵞ) :=
+  ∃ l' : loc, (l +ₗ 1) ↦ # l' ∗ na_ilist (Γᵘ:=[]) p N Φ l'.
+Definition na_ilisti `{!nintpGS Σ} d p N Φ l : iProp Σ :=
+  na_nninv d p N (Φ l) ∗ na_nninv d p N (na_ilisttl p N Φ l).
 Notation na_ilistis := (na_ilisti nderiv).
 
 Section verify.
   Context `{!nintpGS Σ}.
 
   (** [na_ilist] is interpreted into [na_ilisti] *)
-  Fact na_ilist_ilisti {κ p N N' Φ l d} :
-    ⟦ na_ilist p N N' Φ l ⟧{κ}(d) ⊣⊢ na_ilisti d p N N' Φ l.
+  Fact na_ilist_ilisti {κ p N Φ l d} :
+    ⟦ na_ilist p N Φ l ⟧{κ}(d) ⊣⊢ na_ilisti d p N Φ l.
   Proof. by rewrite/= rew_eq_hwf /=. Qed.
 
   (** Convert the predicate of [na_ilisti] *)
-  Lemma na_ilisti_convert `{!nderivy Σ ih d} {p N N' Φ Ψ l} :
+  Lemma na_ilisti_convert `{!nderivy Σ ih d} {p N Φ Ψ l} :
     □ ⸨ ∀ l, (Φ l ={∅}=∗ Ψ l) ∗ (Ψ l ={∅}=∗ Φ l) ⸩(d) -∗
-    na_ilisti d p N N' Φ l -∗ na_ilisti d p N N' Ψ l.
+    na_ilisti d p N Φ l -∗ na_ilisti d p N Ψ l.
   Proof.
     move: d nderivy0 Φ Ψ l. apply (derivy_acc (λ _, ∀ Φ Ψ l, _ -∗ _)).
-    move=> d ? Φ Ψ l. iIntros "#sΦ↔Ψ #[??]".
-    iSplit; iApply na_nninv_convert=>//; iModIntro.
+    move=> d ? Φ Ψ l. iIntros "#sΦ↔Ψ #[ihd itl]".
+    iSplit; iApply na_nninv_convert; [|iApply "ihd"| |iApply "itl"]; iModIntro.
     { iApply derivy_map; [|done]=>/=. iIntros (d' sys' _) "Φ↔Ψ Φ".
       iDestruct ("Φ↔Ψ" $! _) as "[ΦΨ ΨΦ]". iMod ("ΦΨ" with "Φ") as "$".
       iIntros "!> Ψ". by iApply "ΨΦ". }
@@ -53,33 +53,33 @@ Section verify.
   Qed.
 
   (** [na_ilisti] by cons *)
-  Lemma na_ilisti_cons `{!nderivy Σ ih d} {p N N' Φ l l'} :
-    na_nninv d p N (Φ l) -∗ na_ilisti d p N N' Φ l' -∗ (l +ₗ 1) ↦ #l'
-      =[nninv_wsat d]=∗ na_ilisti d p N N' Φ l.
+  Lemma na_ilisti_cons `{!nderivy Σ ih d} {p N Φ l l'} :
+    na_nninv d p N (Φ l) -∗ na_ilisti d p N Φ l' -∗ (l +ₗ 1) ↦ #l'
+      =[nninv_wsat d]=∗ na_ilisti d p N Φ l.
   Proof.
     iIntros "$ #i ↦".
-    iMod (na_nninv_alloc (na_ilisttl _ _ _ _ _) with "[↦]") as "$"; [|done].
+    iMod (na_nninv_alloc (na_ilisttl _ _ _ _) with "[↦]") as "$"; [|done].
     simpl. iExists _. iFrame "↦". by rewrite rew_eq_hwf /=.
   Qed.
 
   (** [na_ilisti] from a one-node loop *)
-  Lemma na_ilisti_loop_1 `{!nderivy Σ ih d} {p N N' Φ l} :
+  Lemma na_ilisti_loop_1 `{!nderivy Σ ih d} {p N Φ l} :
     na_nninv d p N (Φ l) -∗ (l +ₗ 1) ↦ #l =[nninv_wsat d]=∗
-      na_ilisti d p N N' Φ l.
+      na_ilisti d p N Φ l.
   Proof.
     iIntros "#Φ ↦". iFrame "Φ".
-    iMod (na_nninv_alloc_rec (na_ilisttl _ _ _ _ _) with "[↦]") as "$"; [|done].
+    iMod (na_nninv_alloc_rec (na_ilisttl _ _ _ _) with "[↦]") as "$"; [|done].
     iIntros "/= #?". iExists _. rewrite rew_eq_hwf /=. by iFrame "↦ Φ".
   Qed.
 
   (** [na_ilisti] from a two-node loop *)
-  Lemma na_ilisti_loop_2 `{!nderivy Σ ih d} {p N N' Φ l l'} :
+  Lemma na_ilisti_loop_2 `{!nderivy Σ ih d} {p N Φ l l'} :
     na_nninv d p N (Φ l) -∗ na_nninv d p N (Φ l') -∗
     (l +ₗ 1) ↦ #l' -∗ (l' +ₗ 1) ↦ #l =[nninv_wsat d]=∗
-      na_ilisti d p N N' Φ l ∗ na_ilisti d p N N' Φ l'.
+      na_ilisti d p N Φ l ∗ na_ilisti d p N Φ l'.
   Proof.
     iIntros "#Φ #Φ' ↦ ↦'". iFrame "Φ Φ'".
-    iMod (na_nninv_alloc_rec (na_ilisttl _ _ _ _ _ ∗ na_ilisttl _ _ _ _ _)
+    iMod (na_nninv_alloc_rec (na_ilisttl _ _ _ _ ∗ na_ilisttl _ _ _ _)
       with "[↦ ↦']") as "inv"; last first.
     { simpl. by iDestruct (na_nninv_split with "inv") as "[$ $]". }
     iIntros "/= itls". iDestruct (na_nninv_split with "itls") as "[#? #?]".
@@ -87,8 +87,8 @@ Section verify.
   Qed.
 
   (** [siter] terminates under [na_ilistis] *)
-  Lemma twp_siter_na {p N N' Φ E F l} {f : val} {c : nat} : ↑N' ⊆ E → ↑N' ⊆ F →
-    na_ilistis p N N' Φ l -∗
+  Lemma twp_siter_na {p N Φ E F l} {f : val} {c : nat} : ↑N ⊆ E → ↑N ⊆ F →
+    na_ilistis p N Φ l -∗
     (∀ l, [[{ na_nninvd p N (Φ l) ∗ na_own p F }]][nninv_wsatd]
             f #l @ E
           [[{ RET #(); na_own p F }]]) -∗
@@ -109,8 +109,8 @@ Section verify.
   Qed.
 
   (** [siter_nd] terminates under [na_ilistis] *)
-  Lemma twp_siter_nd_na {p N N' Φ E F l} {f : val} : ↑N' ⊆ E → ↑N' ⊆ F →
-    na_ilistis p N N' Φ l -∗
+  Lemma twp_siter_nd_na {p N Φ E F l} {f : val} : ↑N ⊆ E → ↑N ⊆ F →
+    na_ilistis p N Φ l -∗
     (∀ l, [[{ na_nninvd p N (Φ l) ∗ na_own p F }]][nninv_wsatd]
             f #l @ E
           [[{ RET #(); na_own p F }]]) -∗
