nola/examples/logic/verify/vlist.v
@@ -4,33 +4,33 @@ From nola.examples.logic Require Export inv.
 From nola.examples.heap_lang Require Export notation.
 
 (** List whose elements satisfy the pure condition [φ] *)
-Fixpoint vlist {κ Γ} (N N' : namespace) (φ : Z → Prop) (ns : list Z) (l : loc)
+Fixpoint vlist {κ Γ} (N : namespace) (φ : Z → Prop) (ns : list Z) (l : loc)
   : nProp κ Γ :=
   match ns with [] => True | n :: ns =>
     n_inv N (⌜φ n⌝ ∗ l ↦ # n) ∗
-      n_inv N' (∃ l' : loc, (l +ₗ 1) ↦ # l' ∗ vlist N N' φ ns l') end.
+      n_inv N (∃ l' : loc, (l +ₗ 1) ↦ # l' ∗ vlist N φ ns l') end.
 
 (** Interpretaion of [vlist] *)
-Definition vlisti `{!nintpGS Σ} d N N' φ (ns : list Z) l
+Definition vlisti `{!nintpGS Σ} d N φ (ns : list Z) l
   : iProp Σ :=
   match ns with [] => True | n :: ns =>
     nninv d N (⌜φ n⌝ ∗ l ↦ # n) ∗
-      nninv d N' (∃ l' : loc, (l +ₗ 1) ↦ # l' ∗ vlist N N' φ ns l') end.
+      nninv d N (∃ l' : loc, (l +ₗ 1) ↦ # l' ∗ vlist N φ ns l') end.
 Notation vlistis := (vlisti nderiv).
 
 Section verify.
   Context `{!nintpGS Σ}.
 
-  #[export] Instance vlisti_pers {d N N' φ ns l} :
-    Persistent (vlisti d N N' φ ns l).
+  #[export] Instance vlisti_pers {d N φ ns l} :
+    Persistent (vlisti d N φ ns l).
   Proof. case ns; exact _. Qed.
 
-  Lemma vlist_vlisti {κ N N' φ ns l d} :
-    ⟦ vlist N N' φ ns l ⟧{κ}(d) ⊣⊢ vlisti d N N' φ ns l.
+  Lemma vlist_vlisti {κ N φ ns l d} :
+    ⟦ vlist N φ ns l ⟧{κ}(d) ⊣⊢ vlisti d N φ ns l.
   Proof. by case ns. Qed.
 
-  Lemma vlist_all {E N N' φ ns l} : ↑ N ⊆ E → ↑ N' ⊆ E →
-    vlistis N N' φ ns l =[nninv_wsatd]{E}=∗ ⌜Forall φ ns⌝.
+  Lemma vlist_all {E N φ ns l} : ↑ N ⊆ E → ↑ N ⊆ E →
+    vlistis N φ ns l =[nninv_wsatd]{E}=∗ ⌜Forall φ ns⌝.
   Proof.
     move=> ?. move: l. elim ns; [iPureIntro=>/= ??; by apply Forall_nil|].
     iIntros (?? IH ??) "[#ihd #itl]".
